

# ECE203 Mathematical Background

## Preamble

The following are mathematical concepts and questions that are useful and will appear in ECE203. Solving these questions can help you to self-assess your preparation for this course as well as provide a quick reference for a mathematical concept that may need review.

## Questions

1. Let  $q \neq 1$ . Find a simple expression for the sum  $S = \sum_{i=0}^n q^i$ .

*Hint:* What is the product  $(1 - q)(1 + q + q^2 + \cdots + q^n)$ ?

**Solution:** Multiplying out

$$\begin{aligned}(1 - q)(1 + q + q^2 + \cdots + q^n) &= (1 + q + q^2 + \cdots + q^n) - (q + q^2 + \cdots + q^n + q^{n+1}) \\ &= 1 - q^{n+1}\end{aligned}$$

So, dividing both sides by  $(1 - q)$ , we get

$$1 + q + q^2 + \cdots + q^n = \frac{1 - q^{n+1}}{1 - q}$$

2. Let  $-1 < q < 1$ . Use the result of the previous problem to find a simple expression for the sum  $S = \sum_{i=0}^{\infty} q^i$ .

**Solution:**

$$\begin{aligned}S &= \sum_{i=0}^{\infty} q^i \\ &= \lim_{n \rightarrow \infty} \sum_{i=0}^n q^i \\ &= \lim_{n \rightarrow \infty} \frac{1 - q^{n+1}}{1 - q} \\ &= \frac{1}{1 - q}\end{aligned}$$

3. Let  $-1 < q < 1$ . Use the result of the previous problem to find a simple expression for the sum  $S = \sum_{i=1}^{\infty} pq^{i-1}$ .

**Solution:**

$$\begin{aligned}S &= \sum_{i=1}^{\infty} pq^{i-1} && \text{Let } n = i - 1 \\ &= p \sum_{n=0}^{\infty} q^n \\ &= \frac{p}{1 - q}\end{aligned}$$

4. Find a simple expression for  $S = \sum_{i=1}^{\infty} ipq^{i-1}$ .

*Hint:* First i) expand  $i$  into  $i = i - 1 + 1$  and use this to expand the sum into 2 sums. Then ii) make the substitution  $n = i - 1$ , and iii) express the right side in terms of  $S$ . Finally, iv) solve for  $S$ .

**Solution:**

$$\begin{aligned}
 S &= \sum_{i=1}^{\infty} ipq^{i-1} \\
 &= \sum_{i=1}^{\infty} (i-1+1)pq^{i-1} \\
 &= \sum_{i=1}^{\infty} (i-1)pq^{i-1} + \sum_{i=1}^{\infty} pq^{i-1} \\
 &= \sum_{i=1}^{\infty} (i-1)pq^{i-1} + \frac{p}{1-q} \quad \text{Let } n = i-1 \\
 &= \sum_{n=0}^{\infty} npq^n + \frac{p}{1-q} \\
 &= \sum_{n=1}^{\infty} npq^n + \frac{p}{1-q} \quad \text{since } npq^n = 0 \text{ when } n = 0. \\
 &= q \sum_{n=1}^{\infty} npq^{n-1} + \frac{p}{1-q} \\
 &= qS + \frac{p}{1-q}
 \end{aligned}$$

Solving for  $S$ , we get

$$S = \frac{p}{(1-q)^2}$$

5. Recall that the Taylor series of a function  $f(x)$  about  $x = 0$  is

$$f(x) = \sum_{n=0}^{\infty} \frac{f^{(n)}(0)}{n!} x^n$$

where  $f^{(n)}(x)$  is the  $n$ th derivative of  $f(x)$ . Use this to show that

$$\sum_{n=0}^{\infty} \frac{\lambda^n}{n!} e^{-\lambda} = 1$$

**Solution:** Choosing  $f(x) = e^{\lambda x}$ , and computing the first few derivatives:

$$f^{(0)}(0) = f(0) = 1$$

$$f^{(1)}(0) = \lambda e^{\lambda x}|_{x=0} = \lambda$$

$$f^{(2)}(0) = \lambda^2 e^{\lambda x}|_{x=0} = \lambda^2$$

$$f^{(3)}(0) = \lambda^3 e^{\lambda x}|_{x=0} = \lambda^3$$

$\vdots$

$$f^{(n)}(0) = \lambda^n e^{\lambda x}|_{x=0} = \lambda^n$$

So

$$e^{\lambda x} = \sum_{n=0}^{\infty} \frac{\lambda^n}{n!} x^n$$

hence, for  $x = 1$ , we get

$$e^{\lambda} = f(1) = \sum_{n=0}^{\infty} \frac{\lambda^n}{n!}$$

and therefore

$$\sum_{n=0}^{\infty} \frac{\lambda^n}{n!} e^{-\lambda} = e^{-\lambda} \sum_{n=0}^{\infty} \frac{\lambda^n}{n!} = e^{-\lambda} e^{\lambda} = 1$$

6. Find a simple expression for the sum  $S = \sum_{n=0}^{\infty} n \frac{\lambda^n}{n!} e^{-\lambda}$ .

*Hint:* i) Explain why the sum can start at  $n = 1$  instead of  $n = 0$ , ii) then simplify and factor and make the substitution  $m = n - 1$ , iii) apply result of previous problem.

**Solution:**

$$\begin{aligned} S &= \sum_{n=0}^{\infty} n \frac{\lambda^n}{n!} e^{-\lambda} \\ &= \sum_{n=1}^{\infty} n \frac{\lambda^n}{n!} e^{-\lambda} \\ &= \sum_{n=1}^{\infty} \frac{\lambda^n}{(n-1)!} e^{-\lambda} \\ &= \lambda \sum_{n=1}^{\infty} \frac{\lambda^{n-1}}{(n-1)!} e^{-\lambda} \quad \text{Let } m = n - 1 \\ &= \lambda \sum_{m=0}^{\infty} \frac{\lambda^m}{m!} e^{-\lambda} \\ &= \lambda \quad \text{By result of previous problem.} \end{aligned}$$

7. For  $a > 0$ , find a simple expression for the sum  $S = \sum_{n=0}^{\infty} e^{-na}$ .

**Solution:**

$$\begin{aligned} S &= \sum_{n=0}^{\infty} e^{-na} \\ &= \sum_{n=0}^{\infty} (e^{-a})^n \\ &= \frac{1}{1 - e^{-a}} \end{aligned} \quad \text{Since } 0 < e^{-a} < 1$$

8. Expand  $S = \sum_{i=1}^3 \sum_{j=1}^3 a_i b_j$  and verify that  $S = (a_1 + a_2 + a_3)(b_1 + b_2 + b_3)$ .

**Solution:**

$$\begin{aligned} S &= a_1 b_1 + a_1 b_2 + a_1 b_3 + a_2 b_1 + a_2 b_2 + a_2 b_3 + a_3 b_1 + a_3 b_2 + a_3 b_3 \\ &= a_1(b_1 + b_2 + b_3) + a_2(b_1 + b_2 + b_3) + a_3(b_1 + b_2 + b_3) \\ &= (a_1 + a_2 + a_3)(b_1 + b_2 + b_3) \end{aligned}$$

9. Show that in general  $S = \sum_{i=1}^n \sum_{j=1}^m a_i b_j = (\sum_{i=1}^n a_i)(\sum_{j=1}^m b_j)$ .

**Solution:**

$$\begin{aligned} S &= \sum_{i=1}^n \sum_{j=1}^m a_i b_j \\ &= \sum_{i=1}^n (a_i b_1 + a_i b_2 + \cdots + a_i b_m) \\ &= \sum_{i=1}^n [a_i (b_1 + b_2 + \cdots + b_m)] \\ &= a_1(b_1 + b_2 + \cdots + b_m) + a_2(b_1 + b_2 + \cdots + b_m) + \cdots + a_n(b_1 + b_2 + \cdots + b_m) \\ &= (a_1 + a_2 + \cdots + a_n)(b_1 + b_2 + \cdots + b_m) \\ &= \left(\sum_{i=1}^n a_i\right) \left(\sum_{j=1}^m b_j\right) \end{aligned}$$

10. Suppose  $a_{ij} = a_{ji}$ . Expand  $S = \sum_{i=1}^3 \sum_{j=1}^3 a_{ij}$  and verify that  $S = a_{11} + a_{22} + a_{33} + 2[a_{12} + a_{13} + a_{23}]$

**Solution:**

$$\begin{aligned} S &= \sum_{i=1}^3 \sum_{j=1}^3 a_{ij} \\ &= a_{11} + a_{22} + a_{33} + [a_{12} + a_{13} + a_{23}] + [a_{21} + a_{31} + a_{32}] \\ &= a_{11} + a_{22} + a_{33} + 2[a_{12} + a_{13} + a_{23}] \end{aligned} \quad \text{where we used } a_{ij} = a_{ji}$$

11. Suppose  $a_{ij} = a_{ji}$ . Expand  $S = \sum_{i=1}^n \sum_{j=1}^n a_{ij}$  and verify that  $S = \sum_{i=1}^n a_{ii} + 2 \sum_{i < j} a_{ij}$  where the sum over  $i < j$  means the sum over all pairs  $(i, j)$  such that  $1 \leq i < j \leq n$ .

**Solution:** Let

$$B = \{(i, j) \in \mathbb{Z}^2 | 1 \leq i \leq n, 1 \leq j \leq n\}$$

$$C = \{(i, j) \in B | i = j\}$$

$$D = \{(i, j) \in B | i < j\}$$

$$E = \{(i, j) \in B | i > j\}$$

Then  $B = C \cup D \cup E$ , and each  $(i, j)$  pair in  $B$  belongs to only one of  $C$ ,  $D$  or  $E$ . So

$$\begin{aligned} S &= \sum_{i=1}^n \sum_{j=1}^n a_{ij} \\ &= \sum_{(i,j) \in B} a_{ij} \\ &= \sum_{(i,j) \in C} a_{ij} + \sum_{(i,j) \in D} a_{ij} + \sum_{(i,j) \in E} a_{ij} \\ &= \sum_{i=1}^n a_{ii} + \sum_{(i,j) \in D} a_{ij} + \sum_{(i,j) \in E} a_{ij} \\ &=^{(a)} \sum_{i=1}^n a_{ii} + \sum_{(i,j) \in D} a_{ij} + \sum_{(i,j) \in D} a_{ji} \\ &=^{(b)} \sum_{i=1}^n a_{ii} + \sum_{(i,j) \in D} a_{ij} + \sum_{(i,j) \in D} a_{ij} \\ &= \sum_{i=1}^n a_{ii} + 2 \sum_{(i,j) \in D} a_{ij} \\ &= \sum_{i=1}^n a_{ii} + 2 \sum_{i < j} a_{ij} \end{aligned}$$

where (a) follows since we can get the elements of  $E$  by swapping the coordinates of the elements of  $D$ , (b) follows since  $a_{ij} = a_{ji}$ .

12. Compute the derivative of

(a)  $f(x) = x \ln x$

(b)  $f(x) = xe^{ax}$

(c)  $f(x) = e^{1+x^2}$

(d)  $f(x) = (x + \ln x)^n$

(e)  $f(x) = (x^2 e^{bx} + c)^n$

(f)  $f(x) = \int_0^x y^2 dy$

- (g)  $f(x) = \int_{x^2}^x y^2 dy$   
 (h)  $f(x) = \int_{x^2}^x (y+x)^2 dy$

**Solution:**

- (a) Applying the product rule

$$f'(x) = (x)' \ln x + x(\ln x)' = \ln x + x/x = 1 + \ln x$$

- (b) Applying the product rule

$$f'(x) = (x)' e^{ax} + x(e^{ax})' = e^{ax} + axe^{ax}$$

- (c) Applying the chain rule

$$f'(x) = (e^{1+x^2})' = (1+x^2)' e^{1+x^2} = 2xe^{1+x^2}$$

- (d) Applying the chain rule

$$f'(x) = ((x + \ln x)^n)' = n(x + \ln x)^{n-1}(x + \ln x)' = n(x + \ln x)^{n-1}(1 + 1/x)$$

- (e) Applying the chain rule and product rule

$$\begin{aligned} f'(x) &= ((x^2 e^{bx} + c)^n)' \\ &= n(x^2 e^{bx} + c)^{n-1} (x^2 e^{bx} + c)' \\ &= n(x^2 e^{bx} + c)^{n-1} (x^2 e^{bx})' \\ &= n(x^2 e^{bx} + c)^{n-1} ((x^2)' e^{bx} + x^2 (e^{bx})') \\ &= n(x^2 e^{bx} + c)^{n-1} (2xe^{bx} + bx^2 e^{bx}) \end{aligned}$$

- (f) Background: Consider the integral

$$g(x) = \int_{a(x)}^{b(x)} f(x, y) dy$$

When  $x$  increases, there are three sources of change in the value of the integral: i) the lower limit of integration  $a(x)$  can change, the upper limit of integration  $b(x)$  can change, and iii) the integrand  $f(x, y)$  can change. The derivative must account for these 3 sources. Strictly speaking, this problem requires Leibniz's rule, which states that

$$\frac{d}{dx} \int_{a(x)}^{b(x)} f(x, y) dy = b'(x) f(x, b(x)) - a'(x) f(x, a(x)) + \int_{a(x)}^{b(x)} \frac{\partial}{\partial x} f(x, y) dy$$

and each term on the right side above accounts for the three sources of change i), ii) and iii).

Now, back to finding the derivative of  $\int_0^x y^2 dy$ . Applying Leibniz's rule, we get

$$\begin{aligned}\frac{d}{dx}f(x) &= \frac{d}{dx} \int_0^x y^2 dy \\ &= \left[ \frac{d}{dx} x \right] \times [y^2]_{y=x} - \left[ \frac{d}{dx} 0 \right] \times [x^2] - \int_0^x \frac{\partial}{\partial x} y^2 dy \\ &= 1 \times [x^2] - 0 + \int_0^x 0 dy \\ &= x^2\end{aligned}$$

which for this simple problem, you could have obtained by inspection.

(g) Applying Leibniz's rule, we get

$$\begin{aligned}\frac{d}{dx}f(x) &= \frac{d}{dx} \int_{x^2}^x y^2 dy \\ &= \left[ \frac{d}{dx} x \right] \times [y^2]_{y=x} - \left[ \frac{d}{dx} x^2 \right] \times [y^2]_{y=x^2} - \int_{x^2}^x \frac{\partial}{\partial x} y^2 dy \\ &= 1 \times [x^2] - 2x \times x^4 + \int_{x^2}^x 0 dy \\ &= x^2 - 2x^5\end{aligned}$$

An alternate way to get this is by computing the integral:

$$\begin{aligned}\frac{d}{dx}f(x) &= \frac{d}{dx} \int_{x^2}^x y^2 dy \\ &= \frac{d}{dx} [y^3/3]_{x^2}^x \\ &= \frac{d}{dx} [x^3/3 - x^6/3] \\ &= x^2 - 2x^5\end{aligned}$$

(h) Applying Leibniz's rule, we get

$$\begin{aligned}\frac{d}{dx}f(x) &= \frac{d}{dx} \int_{x^2}^x (y+x)^2 dy \\ &= \left[ \frac{d}{dx} x \right] \times [(x+y)^2]_{y=x} - \left[ \frac{d}{dx} x^2 \right] \times [(x+y)^2]_{y=x^2} - \int_{x^2}^x \frac{\partial}{\partial x} (x+y)^2 dy \\ &= 1 \times (x+x)^2 - 2x \times (x+x^2)^2 - \int_{x^2}^x 2(x+y) dy \\ &= 1 \times (x+x)^2 - 2x \times (x+x^2)^2 - 2x \int_{x^2}^x 1 dy - \int_{x^2}^x 2y dy \\ &= 4x^2 - 2x(x+x^2)^2 - 2x[y]_{x^2}^x + [y^2]_{x^2}^x \\ &= 4x^2 - 2x(x+x^2)^2 - 2x(x-x^2) + x^2 - x^4\end{aligned}$$

13. Assume that a function  $F(t)$  has derivative  $f(t)$ , i.e.,

$$\frac{d}{dt}F(t) = f(t).$$

Express the following integrals in terms of  $F(\cdot)$ . If this is not possible, explain why. If the integral does not make sense, explain why.

- (a)  $\int_u^v f(t) dt$
- (b)  $\int_u^v f(t-u) dt$
- (c)  $\int_u^{f(v)-F(u)} f(t-u) dt$
- (d)  $\int_v^{2v} f(t-u) du$
- (e)  $\int_u^v f(ut-u) dt$
- (f)  $\int_0^v f(ut-u) du$
- (g)  $\int_u^v tf(t) dt$
- (h)  $\int_u^t f(t) dt$

**Solution:**

- (a)  $\int_u^v f(t) dt = F(t)|_u^v = F(v) - F(u)$
- (b) Let  $w = t - u$ . Then  $dw = dt$ , and hence

$$\int_u^v f(t-u) dt = \int_0^{v-u} f(w) dw = F(v-u) - F(0),$$

which in hindsight, was obvious, as the original expression is the area under the curve  $f(t)$  between  $t = 0$  and  $t = v - u$ .

- (c) Using the same change of variable as in the previous part,

$$\int_u^{f(v)-F(u)} f(t-u) dt = \int_0^{f(v)-F(u)-u} f(w) dw = F(f(v) - F(u) - u) - F(0).$$

Without knowing anything more about  $f(\cdot)$  or  $F(\cdot)$ , it is impossible to go further.

- (d) The variable of integration is now  $du$ . Using  $w = t - u$  again, we now have  $dw = -du$ . Hence

$$\int_v^{2v} f(t-u) du = \int_{t-v}^{t-2v} f(w) (-dw) = -F(t-2v) + F(t-v)$$

- (e) Using the change of variable  $w = ut - u$ , we have  $dw = u dt$ . Hence

$$\int_u^v f(ut-u) dt = \int_{u^2-u}^{uv-u} f(w) (dw/u) = F(uv-u)/u - F(u^2-u)/u.$$

- (f) Again, the variable of integration is now  $du$ , hence with  $w = ut - u$ , we have  $dw = (t-1)du$ . So

$$\int_0^v f(ut-u) du = \int_0^{vt-v} f(w) dw/(t-1) = F(vt-v)/(t-1) - F(0)/(t-1)$$

- (g) Integrating by parts, we get:

$$\begin{aligned} \int_u^v tf(t) dt &= tF(t)|_u^v - \int_u^v F(t) dt \\ &= vF(v) - uF(u) - \int_u^v F(t) dt \end{aligned}$$

At this point, it depends on whether  $\int_u^v F(t) dt$  is considered an expression in terms of  $F(\cdot)$ . If we don't, then the answer can't be expressed in terms of  $F(\cdot)$ .



- (h) Here, the variable of integration is  $t$ , and one of the limits of integration is also  $t$ . Thus, the integral is not properly posed, and does not strictly make sense. What is most likely intended by such an expression is  $\int_u^t f(w) dw$ , which would be properly posed.

14. Compute the following indefinite integrals

- (a)  $\int e^{ax} dx$
- (b)  $\int xe^{ax} dx$
- (c)  $\int x^2e^{ax} dx$
- (d)  $\int x^3e^{ax} dx$
- (e)  $\int \ln x dx$
- (f)  $\int x \ln x dx$

**Solution:**

- (a) Taking the long approach:

$$\begin{aligned}\int e^{ax} dx &= \frac{1}{a} \int e^u du & u = ax, du = a dx \\ &= \frac{1}{a} e^u\end{aligned}$$

It is customary to add a  $+C$  since adding any constant still results in an anti-derivative.

- (b) We integrate by parts. It is better to derive integration by parts as needed than to try to memorize it. Recall that  $(u(x)v(x))' = u'(x)v(x) + u(x)v'(x)$  so integrating all three terms, we get  $\int u(x)v'(x)dx = u(x)v(x) - \int u'(x)v(x)dx$ .

$$\begin{aligned}\int xe^{ax} dx &= u(x)v(x) - \int u'(x)v(x)dx & u(x) = x, v'(x) = e^{ax}, u'(x) = 1, v(x) = e^{ax}/a \\ &= xe^{ax}/a - \int e^{ax}/a dx \\ &= xe^{ax}/a - e^{ax}/a^2\end{aligned}$$

- (c) We integrate by parts.

$$\begin{aligned}\int x^2e^{ax} dx &= u(x)v(x) - \int u'(x)v(x)dx & u(x) = x^2, v'(x) = e^{ax}, u'(x) = 2x, v(x) = e^{ax}/a \\ &= x^2e^{ax}/a - \int 2xe^{ax}/a dx \\ &= x^2e^{ax}/a - 2 \int xe^{ax}/a dx \\ &= x^2e^{ax}/a - 2(x/a^2)e^{ax} + (2/a^3)e^{ax}\end{aligned}$$

where we used the result from the previous problem in the last step. We could have also gone ahead and integrated by parts a second time.

(d)

$$\begin{aligned}\int x^3 e^{ax} dx &= u(x)v(x) - \int u'(x)v(x)dx & u(x) &= x^3, v'(x) = e^{ax} \\ &= x^3 e^{ax}/a - \int 3x^2 e^{ax}/a dx & u'(x) &= 3x^2, v(x) = e^{ax}/a \\ &= x^3 e^{ax}/a - 3 \int x^2 e^{ax}/a dx \\ &= x^3 e^{ax}/a - (3/a)[x^2 e^{ax}/a - 2(x/a^2)e^{ax} + (2/a^3)e^{ax}] \\ &= x^3 e^{ax}/a - 3x^2 e^{ax}/a^2 + 6(x/a^3)e^{ax} - (6/a^4)e^{ax}\end{aligned}$$

(e)

$$\begin{aligned}\int \ln x dx &= u(x)v(x) - \int u'(x)v(x)dx & u(x) &= \ln x, v'(x) = 1, u'(x) = 1/x, v(x) = x \\ &= x \ln x - \int x/x dx \\ &= x \ln x - x\end{aligned}$$

(f)

$$\begin{aligned}\int x \ln x dx &= u(x)v(x) - \int u'(x)v(x)dx & u(x) &= \ln x, v'(x) = x, u'(x) = 1/x, v(x) = x^2/2 \\ &= (x^2/2) \ln x - \int (x^2/2)/x dx \\ &= (x^2/2) \ln x - x^2/4\end{aligned}$$

15. Let  $A$  be the area given by

$$A = \{(x, y) \in \mathbb{R}^2 | x < 1, y < 1, x + y > 1\}$$

Consider the integral

$$I = \iint_A f(x, y) dx dy$$

Find the limits of integration for this integral when we compute it as an iterated integral with  $x$  integrated in the inner integral, i.e., find  $a, b, c$  and  $d$  in terms of  $x$  and  $y$ :

$$I = \int_a^b \int_c^d f(x, y) dx dy$$

**Solution:** If we plot the area  $A$ , it is triangle formed by the vertices  $(0, 1)$ ,  $(1, 1)$  and  $(1, 0)$ . Since we are integrating with respect to  $x$  first, we must express the limits of integration for  $x$  in terms of  $y$ . The diagonal line from  $(0, 1)$  to  $(1, 0)$  has formula  $x = 1 - y$ .

So, from the region  $A$ ,  $x$  goes from  $1 - y$  to  $1$ . And the  $y$  goes from  $0$  to  $1$ . So

$$I = \int_0^1 \int_{1-y}^1 f(x, y) dx dy$$

16. Express the integral in the previous problem in the form

$$I = \int_a^b \int_c^d f(x, y) dy dx$$

i.e., with  $y$  as the inner integration variable.

**Solution:** The area  $A$  remains the same as before. So the limits for  $y$  need to be expressed in terms of  $x$ . Plotting the region,  $y$  goes from  $1 - x$  to  $1$ , and  $x$  goes from  $0$  to  $1$ , so

$$I = \int_0^1 \int_{1-x}^1 f(x, y) dy dx$$

17. Consider

$$I = \int_0^1 \int_{x^2}^x g(x, y) dy dx$$

Find the limits of integration when we switch the order of integration to  $dx dy$ , i.e., find  $a$ ,  $b$ ,  $c$  and  $d$  in terms of  $x$  and  $y$  such that

$$I = \int_a^b \int_c^d g(x, y) dx dy$$

**Solution:** The region over which the first integral integrates is the region

$$A = \{(x, y) \in \mathbb{R}^2 | x^2 < y < x, 0 < x < 1\}$$

This is the region between  $y = x^2$  and  $y = x$  where  $0 < x < 1$ .

This can equivalently be described as the region between  $x = y$  and  $x = \sqrt{y}$  when  $0 < y < 1$ . So

$$I = \int_0^1 \int_y^{\sqrt{y}} g(x, y) dx dy$$

18. With  $a$ ,  $b$ ,  $c$  and  $d$  as fixed constants, explain why

$$\int_a^b \int_c^d f(x)g(y) dx dy = \int_a^b g(y) dy \int_c^d f(x) dx$$

**Solution:**

$$\begin{aligned} \int_a^b \int_c^d f(x)g(y) dx dy &= \int_a^b g(y) \int_c^d f(x) dx dy && \text{since } g(y) \text{ is constant with respect to } x \\ &= \int_a^b g(y) \left[ \int_c^d f(x) dx \right] dy \\ &= \int_a^b g(y) dy \left[ \int_c^d f(x) dx \right] && \text{since the term in the } [ ] \text{ is a constant} \\ &= \int_a^b g(y) dy \int_c^d f(x) dx \end{aligned}$$